examples/tutorial/5-wp/tutorial_wpScript.sml
@@ -169,6 +169,36 @@ val bir_add_reg_loop_continue_variant_wp_def = Define
 val _ = save_thm ("bir_add_reg_loop_continue_variant_ht", bir_add_reg_loop_continue_variant_ht);
 
 
+(******************     (0) bir_add_reg_mem      ********************)
+(* The WP for the memory part of the add_reg is generated and proved
+ * here. *)
+(* 0 -> 1c *)
+(*
+val prefix = "add_reg_mem_";
+val first_block_label_tm = ``BL_Address (Imm64 0x0w)``; (* 28 *)
+val last_block_label_tm =  ``BL_Address (Imm64 0x1cw)``; (* 64 *)
+val false_label_l = [];
+val postcond_tm = ``bir_add_reg_contract_0_post``;
+(* bir_add_reg_entry_htis the HT stating the generated WP: *)
+
+val defs = [bir_add_reg_prog_def, bir_add_reg_contract_0_post_def, bir_add_reg_contract_0_pre_def];
+
+val bir_add_reg_loop_continue_variant_wp =
+  get_wp_from_ht bir_add_reg_loop_continue_variant_ht;
+val bir_add_reg_loop_continue_variant_wp_def = Define
+  `bir_add_reg_loop_continue_variant_wp v = ^(bir_add_reg_loop_continue_variant_wp)`;
+
+
+val (bir_add_reg_mem_ht, _) =
+  bir_obtain_ht prog_tm first_block_label_tm last_block_label_tm
+                postcond_tm prefix false_label_l defs;
+val bir_add_reg_mem_wp =
+  (rhs o concl o EVAL o (el 4) o snd o strip_comb o concl) bir_add_reg_mem_ht;
+
+val bir_add_reg_mem_wp_def = Define `bir_add_reg_mem_wp = ^(bir_add_reg_mem_wp)`;
+
+val _ = save_thm ("bir_add_reg_mem_ht", bir_add_reg_mem_ht);
+*)
 
 (************           RECENT EXPERIMENTS           **************)
 (* 
@@ -191,10 +221,38 @@ val contract_3_imp =
   prove_imp_w_smt contract_3_pre bir_add_reg_loop_continue_wp;
 
 (* Contract 4 *)
-val contract_4_pre =
-  eot ``bir_add_reg_contract_4_pre``;
-val contract_4_imp =
-  prove_imp_w_smt contract_4_pre bir_add_reg_loop_exit_wp;
+val contract_4_pre = eot ``bir_add_reg_contract_4_pre``;
+val contract_4_imp = prove_imp_w_smt contract_4_pre bir_add_reg_loop_exit_wp;
+*)
+
+(* Contract 0 *)
+(*
+val prefix = "add_reg_mem_";
+val first_block_label_tm = ``BL_Address (Imm64 0x0w)``; (* 28 *)
+val last_block_label_tm =  ``BL_Address (Imm64 0x8w)``; (* 64 *)
+val false_label_l = [];
+val postcond_tm =
+  (snd o dest_eq o concl o EVAL) (btrue);
+val postcond_tm = beq(``(BExp_Load
+                        (BExp_Den (BVar "MEM" (BType_Mem Bit64 Bit8)))
+                        (BExp_BinExp BIExp_Plus
+                           (BExp_Den (BVar "SP_EL0" (BType_Imm Bit64)))
+                           (BExp_Const (Imm64 8w))) BEnd_LittleEndian Bit64)``, get_r0);
+
+
+(* bir_add_reg_entry_htis the HT stating the generated WP: *)
+val (bir_add_reg_mem_ht, _) =
+  bir_obtain_ht prog_tm first_block_label_tm last_block_label_tm
+                postcond_tm prefix false_label_l;
+val bir_add_reg_mem_wp =
+  (rhs o concl o EVAL o (el 4) o snd o strip_comb o concl) bir_add_reg_mem_ht;
+val bir_add_reg_mem_wp_def = Define `bir_add_reg_mem_wp = ^(bir_add_reg_mem_wp)`;
+
+
+val contract_0_pre = (rhs o concl o EVAL) ``bir_add_reg_contract_0_pre``;
+val contract_0_imp = prove_imp_w_smt contract_0_pre bir_add_reg_mem_wp;
+
+Z3_SAT_modelLib.Z3_GET_SAT_MODEL (bir2bool (bimp(contract_0_pre, bir_add_reg_mem_wp)))
 *)
 
 val _ = export_theory();
